-

Cslib/Logics/Propositional/NaturalDeduction/Lemmas.lean
@@ -43,10 +43,10 @@ theorem Theory.le_trans {A B C : Proposition Atom} (hAB : {A} ⊢[T] B)
 theorem Theory.le_antisymm {A B : Proposition Atom} (hAB : {A} ⊢[T] B)
     (hBA : {B} ⊢[T] A) : A ≡[T] B := by grind
 
-theorem Theory.inf_wd (A B A' B' : Proposition Atom) :
-    A ≡[T] A' → B ≡[T] B' → (A ⋏ B) ≡[T] (A' ⋏ B')
+def infWD (A B A' B' : Proposition Atom) :
+    T.equiv A A' → T.equiv B B' → T.equiv (A ⋏ B) (A' ⋏ B')
   | ⟨D,D'⟩, ⟨E,E'⟩ => by
-    constructor; constructor
+    constructor
     · apply conjI
       · refine Theory.Derivation.cut (Γ := {A ⋏ B}) (Δ := ∅) ?_ D
         exact conjE₁ (B := B) <| ass <| by grind
@@ -58,10 +58,14 @@ theorem Theory.inf_wd (A B A' B' : Proposition Atom) :
       · refine Theory.Derivation.cut (Γ := {A' ⋏ B'}) (Δ := ∅) ?_ E'
         exact conjE₂ (A := A') <| ass <| by grind
 
-theorem Theory.sup_wd (A B A' B' : Proposition Atom) :
-    A ≡[T] A' → B ≡[T] B' → (A ⋎ B) ≡[T] (A' ⋎ B')
+theorem Theory.inf_wd (A B A' B' : Proposition Atom) :
+    A ≡[T] A' → B ≡[T] B' → (A ⋏ B) ≡[T] (A' ⋏ B')
+  | ⟨D,D'⟩, ⟨E,E'⟩ => ⟨infWD _ _ _ _ ⟨D,D'⟩ ⟨E,E'⟩⟩
+
+def supWD (A B A' B' : Proposition Atom) :
+    T.equiv A A' → T.equiv B B' → T.equiv (A ⋎ B) (A' ⋎ B')
   | ⟨D,D'⟩, ⟨E,E'⟩ => by
-    constructor; constructor
+    constructor
     · apply disjE (A := A) (B := B) (ass <| by grind)
       · apply disjI₁
         exact D.weak_ctx (by grind)
@@ -72,6 +76,10 @@ theorem Theory.sup_wd (A B A' B' : Proposition Atom) :
         exact D'.weak_ctx (by grind)
       · apply disjI₂
         exact E'.weak_ctx (by grind)
+
+theorem Theory.sup_wd (A B A' B' : Proposition Atom) :
+    A ≡[T] A' → B ≡[T] B' → (A ⋎ B) ≡[T] (A' ⋎ B')
+  | ⟨D,D'⟩, ⟨E,E'⟩ => ⟨supWD _ _ _ _ ⟨D,D'⟩ ⟨E,E'⟩⟩
 
 theorem Theory.inf_le_left {A B : Proposition Atom} : {A ⋏ B} ⊢[T] A :=
   ⟨conjE₁ (B := B) <| ass <| by grind⟩
@@ -100,22 +108,26 @@ theorem Theory.le_top [Inhabited Atom] {A : Proposition Atom} : {A} ⊢[T] ⊤ :
 theorem Theory.bot_le [Bot Atom] {A : Proposition Atom} [IsIntuitionistic T] :
     {⊥} ⊢[T] A := ⟨implE (A := ⊥) (ax <| by grind) (ass <| by grind)⟩
 
-theorem Theory.himp_wd (A B A' B' : Proposition Atom) :
-    A ≡[T] A' → B ≡[T] B' → (A ⟶ B) ≡[T] (A' ⟶ B')
-  | ⟨eA⟩, ⟨eB⟩ => by
-    constructor; constructor
+def himpWD (A B A' B' : Proposition Atom) :
+    T.equiv A A' → T.equiv B B' → T.equiv (A ⟶ B) (A' ⟶ B')
+  | ⟨D,D'⟩, ⟨E,E'⟩ => by
+    constructor
     · apply implI
-      apply mapEquivConclusion _ eB
+      apply mapEquivConclusion _ ⟨E,E'⟩
       apply implE (A := A)
       · exact ass <| by grind
-      · apply mapEquivConclusion _ (commEquiv eA)
+      · apply mapEquivConclusion _ ⟨D',D⟩
         exact ass <| by grind
     · apply implI
-      apply mapEquivConclusion _ (commEquiv eB)
+      apply mapEquivConclusion _ ⟨E',E⟩
       apply implE (A := A')
       · exact ass <| by grind
-      · apply mapEquivConclusion _ eA
+      · apply mapEquivConclusion _ ⟨D,D'⟩
         exact ass <| by grind
+
+theorem Theory.himp_wd (A B A' B' : Proposition Atom) :
+    A ≡[T] A' → B ≡[T] B' → (A ⟶ B) ≡[T] (A' ⟶ B')
+  | ⟨eA⟩, ⟨eB⟩ => ⟨himpWD _ _ _ _ eA eB⟩
 
 theorem Theory.le_himp_iff {A B C : Proposition Atom} :
     {A} ⊢[T] (B ⟶ C) ↔ {A ⋏ B} ⊢[T] C := by
@@ -132,7 +144,7 @@ theorem Theory.le_himp_iff {A B C : Proposition Atom} :
 theorem Theory.compl_wd [Bot Atom] (A A' : Proposition Atom) :
     A ≡[T] A' → (~A) ≡[T] (~A') := (Theory.himp_wd A ⊥ A' ⊥ · (equivalent_refl ⊥))
 
-theorem lem [Bot Atom] [IsClassical T] {A : Proposition Atom} : ⊢[T] (A ⋎ (~A)) := by
+theorem lem [Bot Atom] [IsClassical T] {A : Proposition Atom} : ⊢[T] (A ⋎ ~A) := by
   constructor
   apply implE (A := ~~(A ⋎ ~A)) (ax <| by grind)
   apply implI
@@ -144,5 +156,105 @@ theorem lem [Bot Atom] [IsClassical T] {A : Proposition Atom} : ⊢[T] (A ⋎ (~
   apply implE (A := A ⋎ ~A) (ass <| by grind)
   apply disjI₁
   exact ass <| by grind
+
+/-! ### Negation theorems -/
+
+class PseudoBot (Atom : Type _) where
+  r : Proposition Atom
+
+section Neg
+
+abbrev pseudoNeg [h : PseudoBot Atom] := (· ⟶ h.r)
+
+scoped notation "⊥ᵣ" => PseudoBot.r
+scoped prefix:40 "~ᵣ" => pseudoNeg
+
+instance [Bot Atom] : PseudoBot Atom where
+  r := ⊥
+
+variable [PseudoBot Atom]
+
+def conjNotNotDisj {A B : Proposition Atom} : T.equiv (~ᵣA ⋏ ~ᵣB) (~ᵣ(A ⋎ B)) := by
+  constructor
+  · apply implI
+    apply disjE (A := A) (B := B) (ass <| by grind)
+    · refine implE (A := A) ?_ (ass <| by grind)
+      apply conjE₁ (B := ~ᵣB) (ass <| by grind)
+    · refine implE (A := B) ?_ (ass <| by grind)
+      apply conjE₂ (A := ~ᵣA) (ass <| by grind)
+  · apply conjI
+    · apply implI
+      refine implE (A := A ⋎ B) (ass <| by grind) ?_ --(ass <| by grind)
+      apply disjI₁ <| ass <| by grind
+    · apply implI
+      refine implE (A := A ⋎ B) (ass <| by grind) ?_ --(ass <| by grind)
+      apply disjI₂ <| ass <| by grind
+
+theorem Theory.conj_not_not_disj {A B : Proposition Atom} : (~ᵣA ⋏ ~ᵣB) ≡[T] (~ᵣ(A ⋎ B)) :=
+  ⟨conjNotNotDisj⟩
+
+def notConjOfDisjNot {A B : Proposition Atom} : T.Derivation ⟨{~ᵣA ⋎ ~ᵣB}, ~ᵣ(A ⋏ B)⟩ := by
+  apply implI
+  apply disjE (A := ~ᵣA) (B := ~ᵣB) (ass <| by grind)
+  · apply implE (A := A) (ass <| by grind)
+    apply conjE₁ (B := B) <| ass <| by grind
+  · apply implE (A := B) (ass <| by grind)
+    apply conjE₂ (A := A) <| ass <| by grind
+
+theorem Theory.not_conj_of_disj_not {A B : Proposition Atom} : {~ᵣA ⋎ ~ᵣB} ⊢[T] (~ᵣ(A ⋏ B)) :=
+  ⟨notConjOfDisjNot⟩
+
+def conjDnShift {A B : Proposition Atom} : T.equiv (~ᵣ~ᵣA ⋏ ~ᵣ~ᵣB) (~ᵣ~ᵣ(A ⋏ B)) := by
+  constructor
+  · apply implI
+    apply implE (A := ~ᵣA) (conjE₁ (B := ~ᵣ~ᵣB) <| ass <| by grind)
+    apply implI
+    apply implE (A := ~ᵣB) (conjE₂ (A := ~ᵣ~ᵣA) <| ass <| by grind)
+    apply implI
+    apply implE (A := A ⋏ B) (ass <| by grind)
+    apply conjI <;> exact ass <| by grind
+  · apply conjI
+    · apply implI
+      apply implE (A := ~ᵣ(A ⋏ B)) (ass <| by grind)
+      apply implI
+      apply implE (A := A) (ass <| by grind)
+      exact conjE₁ (B := B) (ass <| by grind)
+    · apply implI
+      apply implE (A := ~ᵣ(A ⋏ B)) (ass <| by grind)
+      apply implI
+      apply implE (A := B) (ass <| by grind)
+      exact conjE₂ (A := A) (ass <| by grind)
+
+def Theory.conj_dn_shift {A B : Proposition Atom} : (~ᵣ~ᵣA ⋏ ~ᵣ~ᵣB) ≡[T] (~ᵣ~ᵣ(A ⋏ B)) :=
+  ⟨conjDnShift⟩
+
+def doubleNegOfSelf {A : Proposition Atom} : T.Derivation ⟨{A},~ᵣ~ᵣA⟩ := by
+  apply implI; apply implE (A := A) <;> exact ass <| by grind
+
+def Theory.Derivation.modusTollens {Γ : Ctx Atom} {A B : Proposition Atom}
+    (D : T.Derivation ⟨insert A Γ, B⟩) : T.Derivation ⟨insert (~ᵣB) Γ, ~ᵣA⟩ := by
+  apply implI; apply implE (A := B) (ass <| by grind); exact D.weak_ctx <| by grind
+
+def tripleNeg {A : Proposition Atom} : T.equiv (~ᵣ~ᵣ~ᵣA) (~ᵣA) :=
+  ⟨doubleNegOfSelf.modusTollens (Γ := ∅), doubleNegOfSelf⟩
+
+def equivNotOfEquiv {A B : Proposition Atom} (e : T.equiv A B) : T.equiv (~ᵣA) (~ᵣB) :=
+  ⟨e.2.modusTollens (Γ := ∅), e.1.modusTollens (Γ := ∅)⟩
+
+def notNotDisjNotOfNotConj {A B : Proposition Atom} :
+    T.equiv (~ᵣ(A ⋏ B)) (~ᵣ~ᵣ(~ᵣA ⋎ ~ᵣB)) := by
+  refine transEquiv (B := ~ᵣ(~ᵣ~ᵣA ⋏ ~ᵣ~ᵣB)) ?_ ?_
+  · refine transEquiv (B := ~ᵣ~ᵣ~ᵣ(A ⋏ B)) ?_ ?_
+    · exact commEquiv tripleNeg
+    · apply equivNotOfEquiv
+      exact commEquiv conjDnShift
+  · apply equivNotOfEquiv
+    exact conjNotNotDisj
+
+
+
+
+
+end Neg
 
 end PL
