Cslib/Logics/Propositional/NaturalDeduction/Monad.lean
@@ -1,0 +1,355 @@
+/-
+Copyright (c) 2025 Thomas Waring. All rights reserved.
+Released under Apache 2.0 license as described in the file LICENSE.
+Authors: Thomas Waring
+-/
+import Cslib.Logics.Propositional.NaturalDeduction.Lemmas
+import Mathlib.Tactic.ITauto
+
+/-! # Double-negative translations via monads
+
+This treatment generalizes the double-negation translations of classical into intuitionistic and
+minimal logic. The rough idea is that the larger logic add a princple of "`f`-elimination", for
+some operator `f` on propositions. Using the properties of this operator (in the cases at hand),
+we can cook up a new translation denoted `(·)ᵒ`, with the properties:
+- `f Aᵒ ≡[T + f-elim] Aᵒ`, for every `A`, and
+- `Γ ⊢[T + f-elim] Bᵒ` implies `Γᵒ ⊢[T] Bᵒ`, so long as `⊢[T] (f A ⟶ A)ᵒ` for each `A`.
+
+The classical case is when `f A = ~~A`, and `Aᵒ` is the "Gödel-Gentzen translation" from classical
+to minimal logic. The difference between IPL and MPL is captured by `f A = A ∪ ⊥`, so that
+`f`-elimination becomes the disjunctive syllogism `A ∪ ⊥ ⟶ A`, which is equivalent to the principle
+of explosion.
+
+Finally, the terminology "monad" is no coincidence here in cslib — this ought to relate to monads
+qua "notions of computation" (Moggi). At very least the two operators mentioned above mimic,
+respectively, continuation-passing style and computations with failiure.
+
+### References
+
+- van den Berg, *A Kuroda-style* j-*translation*,
+<https://link.springer.com/article/10.1007/s00153-018-0656-x>
+- Aczel, *The Russell–Prawitz modality*, <https://doi.org/10.1017/S0960129501003309>
+-/
+
+namespace PL
+
+open Proposition Theory Derivation
+
+variable {Atom : Type _} [DecidableEq Atom] {T : Theory Atom}
+
+/-! ### Monads -/
+
+structure TMonad (T : Theory Atom) where
+  f : Proposition Atom → Proposition Atom
+  map : T.Derivation ⟨{A ⟶ B}, f A ⟶ f B⟩
+  pure (A : Proposition Atom) : T.Derivation ⟨∅, A ⟶ f A⟩
+  join (A : Proposition Atom) : T.Derivation ⟨∅ , f (f A) ⟶ f A⟩
+
+open TMonad
+
+def TMonad.mapDer (t : TMonad T) {A B : Proposition Atom} (D : T.Derivation ⟨{A}, B⟩) :
+    T.Derivation ⟨{t.f A}, t.f B⟩ := by
+  refine implE (A := t.f A) ?_ (ass <| by grind)
+  refine cut (Γ := {t.f A}) (Δ := ∅) (A := A ⟶ B) ?_ ?_
+  · apply implI
+    exact D.weak_ctx (by grind)
+  · exact t.map
+
+def TMonad.pure' (t : TMonad T) (A : Proposition Atom) : T.Derivation ⟨{A}, t.f A⟩ := by
+  apply implE (A := A)
+  · exact t.pure A |>.weak_ctx (by grind)
+  · exact ass <| by grind
+
+def TMonad.preserveEquiv (t : TMonad T) {A B : Proposition Atom} (e : T.equiv A B) :
+    T.equiv (t.f A) (t.f B) := ⟨t.mapDer e.1, t.mapDer e.2⟩
+
+def TMonad.tBind (t : TMonad T) {A B : Proposition Atom} :
+    T.Derivation ⟨{t.f A, A ⟶ t.f B}, t.f B⟩ := by
+  apply implE (A := t.f (t.f B)) (t.join B |>.weak_ctx <| by grind)
+  apply implE (A := t.f A)
+  · exact t.map.weak_ctx <| by grind
+  · exact ass <| by grind
+
+def TMonad.tSeq (t : TMonad T) {A B : Proposition Atom} :
+    T.Derivation ⟨{t.f A, t.f (A ⟶ B)}, t.f B⟩ := by
+  refine Theory.Derivation.cut (Γ := {t.f A, t.f (A ⟶ B)}) (Δ := {t.f (A ⟶ B)})
+    (A := (A ⟶ B) ⟶ t.f B) ?_ ?_ |>.weak_ctx (by grind)
+  · apply implI
+    apply implE (A := t.f A)
+    · exact t.map (A := A) (B := B) |>.weak_ctx (by grind)
+    · exact ass <| by grind
+  · exact t.tBind (A := A ⟶ B) (B := B) |>.weak_ctx (by grind)
+
+def TMonad.tSeq₂ (t : TMonad T) {A B C : Proposition Atom} :
+    T.Derivation ⟨{t.f A, t.f B, t.f (A ⟶ (B ⟶ C))}, t.f C⟩ := by
+  refine Theory.Derivation.cut
+      (Γ := {t.f A, t.f B, t.f (A ⟶ (B ⟶ C))})
+      (Δ := {t.f B})
+      (A := t.f (B ⟶ C)) ?_ (t.tSeq (A := B) (B := C) |>.weak_ctx (by grind))
+    |>.weak_ctx (by grind)
+  · exact t.tSeq (A := A) (B := B ⟶ C) |>.weak_ctx (by grind)
+
+theorem TMonad.map_sDerivable (t : TMonad T) {Γ : Ctx Atom} {B : Proposition Atom} (h : Γ ⊢[T] B) :
+    (Γ.image t.f) ⊢[T] (t.f B) := by
+  induction Γ using Finset.induction generalizing B with
+  | empty =>
+    let ⟨D⟩ := h
+    constructor
+    apply implE (A := B)
+    · exact (t.pure B).weak_ctx <| by grind
+    · exact D.weak_ctx <| by grind
+  | insert A Γ  _ ih =>
+    let ⟨D⟩ := h
+    let ⟨E⟩ := ih ⟨D.implI⟩
+    constructor
+    · rw [Finset.image_insert]
+      refine Theory.Derivation.cut (Γ := Γ.image t.f) (Δ := {t.f A}) (A := t.f (A ⟶ B)) E ?_
+        |>.weak_ctx <| by grind
+      exact t.tSeq (A := A) (B := B) |>.weak_ctx (by grind)
+
+def TMonad.idem (t : TMonad T) (A : Proposition Atom) : T.equiv (t.f A) (t.f (t.f A)) := by
+  constructor
+  · exact implE (A := t.f A) (t.pure (t.f A) |>.weak_ctx <| by grind) (ass <| by grind)
+  · exact implE (A := t.f (t.f A)) (t.join A |>.weak_ctx <| by grind) (ass <| by grind)
+
+def TMonad.equivImplF (t : TMonad T) (A B : Proposition Atom) :
+    T.equiv (A ⟶ t.f B) (t.f (A ⟶ t.f B)) := by
+  constructor
+  · apply implE (A := A ⟶ t.f B)
+    · exact t.pure (A ⟶ t.f B) |>.weak_ctx <| by grind
+    · exact ass <| by grind
+  · apply implI
+    apply implE (A := t.f (t.f B))
+    · exact t.join B |>.weak_ctx <| by grind
+    · refine Theory.Derivation.cut (Γ := {A}) (A := t.f A) (Δ := {t.f (A ⟶ t.f B)}) ?_ t.tSeq
+        |>.weak_ctx (by grind)
+      exact implE (t.pure A |>.weak_ctx (by grind)) (ass <| by grind)
+
+def TMonad.conjShift (t : TMonad T) (A B : Proposition Atom) :
+    T.equiv (t.f (A ⋏ B)) (t.f A ⋏ t.f B) := by
+  constructor
+  · apply conjI   -- this direction only uses functoriality
+    · apply t.mapDer; exact conjE₁ (B := B) <| ass <| by grind
+    · apply t.mapDer; exact conjE₂ (A := A) <| ass <| by grind
+  · refine implE (A := t.f B) (implE (A := t.f A) ?_ ?_) ?_
+    · apply implI; apply implI
+      apply implE (A := t.f (A ⟶ (B ⟶ (A ⋏ B))))
+      · apply implI
+        exact t.tSeq₂ (A := A) (B := B) (C := A ⋏ B) |>.weak_ctx <| by grind
+      · apply implE (A := A ⟶ (B ⟶ (A ⋏ B))) (t.pure (A ⟶ (B ⟶ (A ⋏ B))) |>.weak_ctx <| by grind)
+        apply implI; apply implI
+        apply conjI <;> exact ass <| by grind
+    · exact conjE₁ (B := t.f B) <| ass <| by grind
+    · exact conjE₂ (A := t.f A) <| ass <| by grind
+
+def TMonad.disjShift (t : TMonad T) (A B : Proposition Atom) :
+    T.equiv (t.f (A ⋎ B)) (t.f (t.f A ⋎ t.f B)) := by
+  constructor
+  · apply t.mapDer
+    apply disjE (A := A) (B := B) (ass <| by grind)
+    · apply disjI₁
+      exact t.pure' A |>.weak_ctx (by grind)
+    · apply disjI₂
+      exact t.pure' B |>.weak_ctx (by grind)
+  · refine Theory.Derivation.cut (Γ := ∅) (Δ := {t.f (t.f A ⋎ t.f B)})
+        (A := t.f A ⋎ t.f B ⟶ t.f (A ⋎ B)) ?_ ?_
+    · apply implI
+      apply disjE (A := t.f A) (B := t.f B) (ass <| by grind)
+      · let : T.Derivation ⟨{A}, A ⋎ B⟩ := disjI₁ <| ass (by grind)
+        exact t.mapDer this |>.weak_ctx (by grind)
+      · let : T.Derivation ⟨{B}, A ⋎ B⟩ := disjI₂ <| ass (by grind)
+        exact t.mapDer this |>.weak_ctx (by grind)
+    · exact t.tBind (A := t.f A ⋎ t.f B) (B := A ⋎ B) |>.weak_ctx (by grind)
+
+/-! ### *j*-Translation -/
+
+/-- Gödel-Gentzen style translation. -/
+@[reducible]
+def TMonad.gg (t : TMonad T) : Proposition Atom → Proposition Atom
+  | atom x => t.f (atom x)
+  | conj A B => conj (t.gg A) (t.gg B)
+  | disj A B => t.f <| disj (t.gg A) (t.gg B)
+  | impl A B => impl (t.gg A) (t.gg B)
+
+def TMonad.ggActionEquiv (t : TMonad T) :
+    (A : Proposition Atom) → T.equiv (t.f <| t.gg A) (t.gg A)
+  | atom x => commEquiv <| t.idem <| atom x
+  | conj A B => by
+    refine transEquiv (B := t.f (t.gg A) ⋏ t.f (t.gg B)) ?_ ?_
+    · exact t.conjShift (t.gg A) (t.gg B)
+    · exact infWD _ _ _ _ (t.ggActionEquiv A) (t.ggActionEquiv B)
+  | disj A B => commEquiv <| t.idem _
+  | impl A B => by
+    let eA := t.ggActionEquiv A
+    let eB := t.ggActionEquiv B
+    constructor
+    · apply implI
+      apply mapEquivHypothesis {t.f (t.gg A ⟶ t.gg B)} eA
+      apply mapEquivConclusion _ eB
+      exact t.tSeq
+    · apply implE (A := t.gg A ⟶ t.gg B)
+      · exact t.pure (t.gg A ⟶ t.gg B) |>.weak_ctx (Finset.empty_subset _)
+      · exact ass <| by exact Finset.mem_singleton.mpr rfl
+
+def TMonad.preserveDerivation (t : TMonad T) {T' : Theory Atom}
+    (derT' : ∀ A ∈ T', T.Derivation ⟨∅, t.gg A⟩) {Γ : Ctx Atom} {B : Proposition Atom} :
+      T'.Derivation ⟨Γ, B⟩ → T.Derivation ⟨Γ.image t.gg, t.gg B⟩
+  | ax hB => (derT' B hB).weak_ctx <| Finset.empty_subset _
+  | ass hB => ass (by grind)
+  | conjI D E => conjI (t.preserveDerivation derT' D) (t.preserveDerivation derT' E)
+  | conjE₁ D => conjE₁ (t.preserveDerivation derT' D)
+  | conjE₂ D => conjE₂ (t.preserveDerivation derT' D)
+  | @disjI₁ _ _ _ _ A B D => by
+    apply implE (A := (t.gg A ⋎ t.gg B))
+    · exact t.pure (t.gg A ⋎ t.gg B) |>.weak_ctx (by grind)
+    · exact disjI₁ (t.preserveDerivation derT' D)
+  | @disjI₂ _ _ _ _ A B D => by
+    apply implE (A := (t.gg A ⋎ t.gg B))
+    · exact t.pure (t.gg A ⋎ t.gg B) |>.weak_ctx (by grind)
+    · exact disjI₂ (t.preserveDerivation derT' D)
+  | @disjE _ _ _ _ A B C D E E' => by
+    apply mapEquivConclusion _ (t.ggActionEquiv C)
+    refine cut (Γ := Γ.image t.gg) (Δ := Γ.image t.gg) (A := t.f (t.gg A ⋎ t.gg B))
+      (t.preserveDerivation derT' D) ?_ |>.weak_ctx (by grind)
+    refine cut (Γ := Γ.image t.gg) (Δ := {t.f <| (t.gg A) ⋎ (t.gg B)})
+        (A := (t.gg A) ⋎ (t.gg B) ⟶ t.f (t.gg C)) ?_ ?_ |>.weak_ctx (by grind)
+    · apply implI
+      apply mapEquivConclusion _ (commEquiv <| t.ggActionEquiv C)
+      apply disjE (A := t.gg A) (B := t.gg B) (ass <| by grind)
+      · exact (t.preserveDerivation derT' E).weak_ctx <| by grind
+      · exact (t.preserveDerivation derT' E').weak_ctx <| by grind
+    · exact t.tBind (A := t.gg A ⋎ t.gg B) (B := t.gg C) |>.weak_ctx (by grind)
+  | implI _ D => implI (Γ.image t.gg) (Finset.image_insert t.gg _ Γ ▸ t.preserveDerivation derT' D)
+  | implE D E => implE (t.preserveDerivation derT' D) (t.preserveDerivation derT' E)
+
+theorem TMonad.preserve_derivability (t : TMonad T) {T' : Theory Atom}
+    (derT' : ∀ A ∈ T', ⊢[T] t.gg A) {Γ : Ctx Atom} {B : Proposition Atom} :
+    Γ ⊢[T'] B → (Γ.image t.gg) ⊢[T] t.gg B
+  | ⟨D⟩ => ⟨t.preserveDerivation (fun A hA => Classical.choice <| derT' A hA) D⟩
+
+@[reducible]
+def TMonad.TElim (t : TMonad T) : Theory Atom := Set.range (fun A => t.f A ⟶ A)
+
+/-! TODO: all of these results actually apply to `T'` such that `T ∪ t.TElim ≤ T'`. -/
+
+def TMonad.actionTrivOfTElim (t : TMonad T) (A : Proposition Atom) :
+    (T ∪ t.TElim).equiv A (t.f A) := by
+  constructor
+  · apply implE (A := A)
+    · apply (t.pure A).weak <;> grind
+    · exact ass <| by grind
+  · exact implE (A := t.f A) (ax <| by grind) (ass <| by grind)
+
+def TMonad.ggEquiv (t : TMonad T) : (A : Proposition Atom) → (T ∪ t.TElim).equiv A (t.gg A)
+  | atom x => t.actionTrivOfTElim (atom x)
+  | conj A B => infWD _ _ _ _ (t.ggEquiv A) (t.ggEquiv B)
+  | disj A B => by
+    refine transEquiv (B := t.gg A ⋎ t.gg B) ?_ ?_
+    · apply supWD <;> exact t.ggEquiv _
+    · exact t.actionTrivOfTElim _
+  | impl A B => himpWD _ _ _ _ (t.ggEquiv A) (t.ggEquiv B)
+
+theorem TMonad.derivable_tElim_iff (t : TMonad T) (hT : ∀ A ∈ T, ⊢[T] t.gg A)
+    (h : ∀ A : Proposition Atom, ⊢[T] t.gg (t.f A ⟶ A)) :
+    Γ ⊢[T ∪ t.TElim] B ↔ (Γ.image t.gg) ⊢[T] (t.gg B) := by
+  constructor <;> intro h_der
+  · refine t.preserve_derivability (T' := T ∪ t.TElim) ?_ h_der
+    intro A hA
+    rw [Set.mem_union, Set.mem_range] at hA
+    cases hA
+    case inl hA => exact hT A hA
+    case inr hA =>
+      replace ⟨A', hA⟩ := hA
+      rw [← hA]
+      exact h A'
+  · induction Γ using Finset.induction generalizing B with
+    | empty =>
+      refine (((T ∪ t.TElim).equiv_iff_equiv_conclusion (A := t.gg B) (B := B)).mp ?_ <|
+          (∅ : Ctx Atom)).mp ?_
+      · exact ⟨commEquiv (t.ggEquiv B)⟩
+      · exact h_der.weak_theory (by grind)
+    | insert A Γ _ ih =>
+      suffices (T ∪ t.TElim).SDerivable ⟨Γ, A ⟶ B⟩ by
+        let ⟨D⟩ := this
+        exact ⟨implE (A := A) (D.weak_ctx <| by grind) (ass <| by grind)⟩
+      apply ih (B := A ⟶ B)
+      let ⟨D⟩ := h_der
+      exact ⟨implI _ <| (Finset.image_insert t.gg _ _) ▸ D⟩
+
+
+/-! ### Examples -/
+
+section PseudoNeg
+
+variable [PseudoBot Atom]
+
+def mapDN {A B : Proposition Atom} : T.Derivation ⟨{A ⟶ B}, ~ᵣ~ᵣA ⟶ ~ᵣ~ᵣB⟩ := by
+  apply implI; apply implI
+  apply implE (A := ~ᵣA) (ass <| by grind)
+  apply implI
+  apply implE (A := B) (ass <| by grind)
+  apply implE (A := A) <;> exact ass (by grind)
+
+def pureDN (A : Proposition Atom) : T.Derivation ⟨∅, A ⟶ ~ᵣ~ᵣA⟩ := by
+  apply implI; apply implI
+  apply implE (A := A) <;> exact ass <| by grind
+
+def joinDN (A : Proposition Atom) : T.Derivation ⟨∅, ~ᵣ~ᵣ~ᵣ~ᵣA ⟶ ~ᵣ~ᵣA⟩ := implI _ tripleNeg.1
+
+def DN : (TMonad T) where
+  f := (~ᵣ~ᵣ ·)
+  map := mapDN
+  pure := pureDN
+  join := joinDN
+
+def mapOrB {A B : Proposition Atom} : T.Derivation ⟨{A ⟶ B}, (A ⋎ ⊥ᵣ) ⟶ (B ⋎ ⊥ᵣ)⟩ := by
+  apply implI
+  apply disjE (A := A) (B := ⊥ᵣ) (ass <| by grind)
+  · apply disjI₁; apply implE (A := A) <;> exact ass <| by grind
+  · apply disjI₂; exact ass (by grind)
+
+def pureOrB (A : Proposition Atom) : T.Derivation ⟨∅, A ⟶ A ⋎ ⊥ᵣ⟩ :=
+  implI _ <| disjI₁ <| ass <| by grind
+
+def joinOrB (A : Proposition Atom) : T.Derivation ⟨∅, (A ⋎ ⊥ᵣ) ⋎ ⊥ᵣ ⟶ A ⋎ ⊥ᵣ⟩ := by
+  apply implI
+  apply disjE (A := A ⋎ ⊥ᵣ) (B := ⊥ᵣ) (ass <| by grind) (ass <| by grind)
+  apply disjI₂; exact ass <| by grind
+
+def OrB : (TMonad T) where
+  f := (· ⋎ ⊥ᵣ)
+  map := mapOrB
+  pure := pureOrB
+  join := joinOrB
+
+def mapPierce {A B : Proposition Atom} :
+    T.Derivation ⟨{A ⟶ B}, (~ᵣA ⟶ A) ⟶ (~ᵣB ⟶ B)⟩ := by
+  apply implI; apply implI
+  apply implE (A := A) (ass <| by grind)
+  apply implE (A := ~ᵣA) (ass <| by grind)
+  apply implI
+  apply implE (A := B) (ass <| by grind)
+  apply implE (A := A) <;> exact ass <| by grind
+
+def purePierce (A : Proposition Atom) : T.Derivation ⟨∅, A ⟶ (~ᵣA ⟶ A)⟩ :=
+  implI _ <| implI _ <| ass <| by grind
+
+def joinPierce (A : Proposition Atom) :
+    T.Derivation ⟨∅, (~ᵣ(~ᵣA ⟶ A) ⟶ (~ᵣA ⟶ A)) ⟶ (~ᵣA ⟶ A)⟩ := by
+  apply implI; apply implI
+  refine implE (A := ~ᵣA) ?_ (ass <| by grind)
+  apply implE (A := ~ᵣ(~ᵣA ⟶ A)) (ass <| by grind)
+  apply implI
+  apply implE (A := A)
+  · exact ass <| by grind
+  · apply implE (A := ~ᵣA) <;> exact ass <| by grind
+
+def Pierce : (TMonad T) where
+  f A := ~ᵣA ⟶ A
+  map := mapPierce
+  pure := purePierce
+  join := joinPierce
+
+end PseudoNeg
+
+end PL
